EventStructures2.thy
@@ -2,29 +2,23 @@ theory EventStructures2
 imports Main Relation
 begin
 
+datatype mem_action = W | R | I   
+datatype label = Label mem_action string int
+
+type_synonym 'a config = "'a set"
+  
 locale partial_order =
   fixes preceeds :: "'a \<Rightarrow> 'a \<Rightarrow> bool" (infixl "\<preceq>" 50)
-  fixes events :: "'a set" ("\<EE>" 1000)
+    and events :: "'a set" ("\<EE>" 1000)
   assumes refl [intro, simp]: "x \<preceq> x"
     and anti_sym [intro]: "\<lbrakk> x \<preceq> y; y \<preceq> x \<rbrakk> \<Longrightarrow> x = y"
     and trans [trans]: "\<lbrakk> x \<preceq> y; y \<preceq> z \<rbrakk> \<Longrightarrow> x \<preceq> z"
 
-locale primeES = partial_order + 
+locale labelledES = partial_order + 
   fixes conflict :: "'a \<Rightarrow> 'a \<Rightarrow> bool" (infixl "#" 50)
+    and label :: "'a \<Rightarrow> label"
   assumes sym [intro]: "\<lbrakk> conflict x y \<rbrakk> \<Longrightarrow> conflict y x"
     and confOverPO [intro]: "\<lbrakk> conflict c d; d \<preceq> e \<rbrakk> \<Longrightarrow> conflict c e"
-
-datatype mem_action = W | R | I   
-datatype label = Label mem_action string int
-type_synonym 'a config = "'a set"
-
-locale labelledES = primeES + 
-  fixes label :: "'a \<Rightarrow> label"
-  fixes config_domain :: "'a config set" ("\<CC>" 1000)
-  assumes conflict_free: "\<lbrakk>C \<in> config_domain; x \<in> C; y \<in> C \<rbrakk> \<Longrightarrow> \<not>(conflict x y)"
-    and down_closed: "\<lbrakk>C \<in> config_domain; y \<in> C; x \<preceq> y \<rbrakk> \<Longrightarrow> x \<in> C"
-    and config_subset: "C \<in> \<CC> \<Longrightarrow> C \<subseteq> \<EE>"
-
 
 
 end
