ExampleEventStructures.thy
@@ -2,31 +2,57 @@ theory ExampleEventStructures
 imports Enum EventStructures Relation Transitive_Closure String
 begin
 
-theorem emptyESValidES: "isValidES \<I>"
-  apply(auto simp add: isValidES_def initialES_def isValidPO_def minimal_def isConfValid_def)
-  apply(rule refl_Id)
-     apply(rule trans_Id)
-    apply(rule antisym_Id)
-   apply(simp add: symmetriccl_def symmetric_symmetriccl)
-   apply(simp add: sym_def trans_def irrefl_def)
-  apply(simp add: trans_rtrancl)
+interpretation emptyES: labelledES 
+  "\<lambda>x y . (x, y) \<in> {(1,1)}\<^sup>*"  -- Order
+  "{1}" -- Events
+  "\<lambda>x y . (x, y) \<in> {}" -- Conflict
+  "\<lambda>x . Label I '''' 0" -- Labelling
+  apply(unfold_locales) 
+         apply(auto)
+   apply (metis Domain_empty Domain_insert Not_Domain_rtrancl singleton_iff)
   done
-    
-lemma initialConfig_no_read: "\<not> is_read x \<I>"
-  apply(simp add: initialES_def)
-  apply(simp add: is_read_def)
+      
+thm labelledES.well_justified_def    
+thm labelledES.config_domain_def
+thm mem_Collect_eq[where P="\<lambda>C . emptyES.conflict_free C \<and> emptyES.down_closed C"]
+  
+lemma (in labelledES) "emptyES.well_justified {}"
+  apply(simp only: emptyES.well_justified_def)
+  apply (rule conjI)
+  using emptyES.justified_def apply blast
+  apply(rule conjI)
+   apply(simp only: emptyES.config_domain_def)
+   apply(simp only: mem_Collect_eq)
+   apply(auto simp only: emptyES.conflict_free_def)
+   apply(auto simp only: emptyES.down_closed_def)
+   apply(simp only: emptyES.ae_justifies_subset_star_def)
   done
-    
-theorem emptyESWellJustified: "well_justified \<I> \<C>"
-  apply(auto simp add: well_justified_def)
-  apply(rule emptyESValidES)
-   apply(auto simp add: justified_def ae_justifies_subset_star_def)
-  done
-    
-    
-theorem emptyESJustEmptyES: "{} \<lesssim>\<^bsub>es\<^esub> {}"
-  apply(auto simp add: justifies_config_inf_def justifies_config_subset_def justifies_config_def)
-  done
-    
+    (*
+    theorem emptyESValidES: "isValidES"
+      apply(auto simp add: isValidES_def initialES_def isValidPO_def minimal_def isConfValid_def)
+      apply(rule refl_Id)
+         apply(rule trans_Id)
+        apply(rule antisym_Id)
+       apply(simp add: symmetriccl_def symmetric_symmetriccl)
+       apply(simp add: sym_def trans_def irrefl_def)
+      apply(simp add: trans_rtrancl)
+      done
+        
+    lemma initialConfig_no_read: "\<not> is_read x"
+      apply(simp add: is_read_def)
+      done
+        
+    theorem emptyESWellJustified: "well_justified \<I> \<C>"
+      apply(auto simp add: well_justified_def)
+      apply(rule emptyESValidES)
+       apply(auto simp add: justified_def ae_justifies_subset_star_def)
+      done
+        
+        
+    theorem emptyESJustEmptyES: "{} \<lesssim>\<^bsub>es\<^esub> {}"
+      apply(auto simp add: justifies_config_inf_def justifies_config_subset_def justifies_config_def)
+      done
+    *)
+  end
 end
   
